# Cubic equation

	a*x^3 + b*x^2 + c*x + d = 0

	p = (3*a*c - b^2)/
		/(3*a^2)
	q = (2*b^3 - 9*a*b*c + 27*a^2*d)/
		/(27*a^3)

	x = y - b/(3*a)
	y^3 + p*y + q = 0
	▲
		a*(y - b/(3*a))^3 +
		+ b*(y - b/(3*a))^2 +
		+ c*(y - b/(3*a)) + d = 
		= a*(y^3 - y^2*b/a + y*b^2/3/a^2 - b^3/27/a^3) +
		+ b*(y^2 - 2*y*b/3/a + b^2/9/a^2) +
		+ c*(y - b/(3*a)) + d =
		= a*y^3 - y^2*b + y*b^2/3/a - b^3/27/a^2 +
		+ y^2*b - 2*y*b^2/3/a + b^3/9/a^2 +
		+ c*y - b*c/3/a + d =
		= a*y^3 - b^3/27/a^2 +
		+ b^3/9/a^2 - y*b^2/3/a +
		+ c*y - b*c/3/a + d
		
		y^3 - b^3/27/a^3 +
		+ b^3/9/a^3 - y*b^2/3/a^2 +
		+ y*c/a - b*c/3/a^2 + d/a =
		= y^3 + y*(c/a - b^2/3/a^2) +
		+ (b^3/9/a^3 - b^3/27/a^3 - b*c/3/a^2 + d/a) =
		= y^3 + y*p + q = 0

		p = c/a - b^2/3/a^2 = (3*a*c - b^2)/(3*a^2)
		q = b^3/9/a^3 - b^3/27/a^3 - b*c/3/a^2 + d/a =
		= (b^3/9/a - b^3/27/a^2 - b*c/3/a + d)/a =
		= (3*b^3* - b^3 - 9*a*b*c + 27*a^2*d)/(27*a^3)
	∎


	y = t - (p/3t)
	t^3 - p^3/(27*t^3) + q = 0
	t^6 + q*t^3 - p^3/27 = 0

